\documentclass{report}

\input{mytemplate}

\title{Midterm Exams Reviewer}
\author{Raphael Lontoc}
\date{October 2024}

\begin{document}

\maketitle

\chapter*{Variable Separable ODE}

\prob{}{
    Solve $(1+x) dy - y dx = 0$
}
\soln Dividing by $(1+x)y$, we get
\[
    \frac{dy}{y} = \frac{dx}{1+x}
\]
from which it follows that
\begin{align*}
    \int \frac{dy}{y} &= \int \frac{dx}{1+x} \\
    \ln|y| &= \ln|1+x| + c \\ 
    e^{\ln|y|} &= e^{\ln|1+x| + c} \\
    y &= e^c(1+x)
\end{align*}
Relabeling the $e^c$ as $c$ then gives us
\[
    y=c(1+x)
\]
\ans $y=c(1+x)$

\medskip

\prob{}{
    Solve $\frac{dy}{dx}=-\frac{x}{y}$
}
\soln Multiplying $y dx$, we get
\[
    y dy = -x dx
\]
and integrating both sides gives us
\begin{align*}
    \int y dy &= \int -x dx \\
    \frac{y^2}{2} &= -\frac{x^2}{2} + c
\end{align*}
Solving for $y$ gives us
\[
    y = \pm\sqrt{-x^2+2c}
\]
\ans $y = \pm\sqrt{-x^2+2c}$

\medskip

\prob{}{
    Solve $\frac{dy}{dx}=e^{3x+2y}$
}
\soln Rewriting $e^3x+2y$ as $e^{3x}e^{2y}$, we get
\[
    \frac{dy}{dx} = e^{3x}e^{2y}
\]
Dividing by $e^2y dx$ we get
\[
    \frac{dy}{e^{2y}} = e^{3x}dx
\]
and integrating both sides gives us
\begin{align*}
    \int \frac{dy}{e^{2y}} &= \int e^{3x}dx \\
    -\frac{1}{2}e^{-2y} &= \frac{1}{3}e^{3x} + c \\
    3e^{-2y} &= -2e^{3x} + c
\end{align*}
\ans $3e^{-2y} = -2e^{3x} + c$

\pagebreak

\chapter*{Homogeneous ODE}

\prob{}{
    Solve $2x^3ydx+(x^4+y^4)dy=0$
}
\soln Each coefficient is a homogeneous function of degree four, so we can let $x=vy$ and substitute to get
\begin{align*}
    2(vy)^3yd(vy)+((vy)^4+y^4)dy &= 0 \\
    2v^3y^4(vdy+ydv)+(v^4y^4+y^4)dy &= 0 \\
    2v^4y^4dy+2v^3y^5dv+v^4y^4dy+y^4dy &= 0 \\
    3v^4y^4dy+2v^3y^5dv+y^4dy &= 0 \\
    y^4(3v^4+1)dy+2v^3y^5dv &= 0
\end{align*}
Now we can separate the variables and integrate to get
\begin{align*}
    \int \frac{dy}{y} + \int \frac{2v^3}{3v^4+1}dv &= \int 0 \\
    \ln{|y|} + \frac{1}{6}\ln{|3v^4+1|} &= c \\
    6\ln{|y|} + \ln{|3v^4+1|} &= c \\
    e^{6\ln{|y|}}+e^{\ln{|3v^4+1|}} &= e^c \\
    y^6+(3v^4+1) &= c \\
    y^6+\frac{3x^4}{y^4}+1 &= c \\
    y^6+\frac{3x^4}{y^4} &= c-1 \\
\end{align*}
Rewriting $c-1$ as $c$, we get
\[
    y^6+\frac{3x^4}{y^4} = c
\]
\ans $y^6+\frac{3x^4}{y^4} = c$

\medskip

\prob{}{
    Solve $(x^2+y^2)dx+(x^2-xy)dy=0$
}
\soln Both $M(x,y)$ and $N(x,y)$ are homogeneous functions of degree two, so we can let $y=ux$ and substitute to get

\begin{align*}
    (x^2+(ux)^2)dx+(x^2-(ux)^2)d(ux) &= 0 \\
    (x^2+u^2x^2)dx+(x^2-u^2x^2)[udx+xdu] &= 0 \\
    x^2dx+u^2x^2dx+ux^2dx+x^3du-u^3x^2dx-u^2x^3du &= 0 \\
    x^2(1+u)dx+x^3(1-u)du &= 0
\end{align*}

Now we can separate the variables and integrate to get

\begin{align*}
    \frac{dx}{x}+\frac{1-u}{1+u}du &= 0 \\
    \frac{dx}{x}+[-1+\frac{2}{1+u}]du &= 0 \\
    \int \frac{dx}{x}+\int [-1+\frac{2}{1+u}]du &= \int 0 \\
    \ln{|x|}-u+2\ln{|1+u|} &= c \\
    \ln{|x|}+\frac{y}{x}-2\ln{|1+\frac{y}{x}|} = c
\end{align*}

We can rewrite c as $\ln{c}$, and then using the properties of logarithms, we can get

\[
    ln{\frac{(x+y)^2}{cx}} = \frac{y}{x}
\]

The definition of logarithms then yeilds

\[
    (x+y)^2 = cxe^\frac{y}{x}
\]

\ans $(x+y)^2 = cxe^\frac{y}{x}$

\medskip

\prob{}{
    Solve $(x-y)dx+xdy=0$
}

The 

\end{document}